books/projects/x86isa/machine/instructions/fp/x86-fp-bitscan-instructions.lisp
@@ -15,36 +15,48 @@
 ; INSTRUCTION: Bit Scan
 ; =============================================================================
 
-(encapsulate
- ()
+(define bsf ((index natp)
+             (x natp))
+  :returns (index natp :hyp (natp index)
+                  :rule-classes :type-prescription)
+  :prepwork
+  ((local
+    (in-theory (e/d* (bitops::ihsext-inductions bitops::ihsext-recursive-redefs)
+                     ()))))
+  (if (zp x)
+      0
+    (if (equal (loghead 1 x) 1)
+        index
+      (bsf (1+ index) (logtail 1 x))))
 
- (local (in-theory (e/d* (ihsext-inductions
-                          ihsext-recursive-redefs)
-                         ())))
+  ///
 
- (define bsf ((index natp)
-              (x natp))
-   :hints (("Goal" :in-theory (enable logtail)))
-   :returns (index natp :hyp (natp index)
-                   :rule-classes :type-prescription)
-   (if (zp x)
-       0
-     (if (logbitp 0 x)
-         index
-       (bsf (1+ index) (ash x -1))))
-   ///
-   (defthm bsf-64
-     (implies (n64p x)
-              (< (bsf 0 x) 64))
-     :rule-classes :linear)))
+  (defthm bsf-zero
+    (equal (bsf index 0) 0))
+
+  (defthm bsf-posp-strict-lower-bound
+    (implies (and (posp x) (natp index))
+             (<= index (bsf index x)))
+    :rule-classes :linear)
+
+  (defthm bsf-posp-strict-upper-bound
+    (implies (and (posp x) (natp index))
+             (<= (bsf index x) (+ -1 (integer-length x) index)))
+    :rule-classes :linear)
+
+  (defthm bsf-64
+    (implies (unsigned-byte-p 64 x)
+             (< (bsf 0 x) 64))
+    :hints (("Goal"
+             :cases ((zp x))
+             :in-theory (e/d* () (bsf unsigned-byte-p))))
+    :rule-classes :linear))
 
 (def-inst x86-bsf-Op/En-RM
 
   :parents (two-byte-opcodes fp-opcodes)
   :implemented
-  (progn
-    (add-to-implemented-opcodes-table 'BSF #x0FBC '(:nil nil) 'x86-bsf-Op/En-RM)
-    (add-to-implemented-opcodes-table 'BSF #x0FBC '(:misc (logbitp *w* rex-byte)) 'x86-bsf-Op/En-RM))
+  (add-to-implemented-opcodes-table 'BSF #x0FBC '(:nil nil) 'x86-bsf-Op/En-RM)
 
   :short "Bit scan forward"
 
@@ -91,9 +103,8 @@
             (the (integer 0 4) increment-RIP-by)
             (the (signed-byte 64) ?v-addr)
             x86)
-        (x86-operand-from-modr/m-and-sib-bytes #.*rgf-access* operand-size
-                                               p2 p4? temp-rip
-                                               rex-byte r/m mod sib 0 x86))
+        (x86-operand-from-modr/m-and-sib-bytes
+         #.*rgf-access* operand-size p2 p4? temp-rip rex-byte r/m mod sib 0 x86))
 
        ((when flg0)
         (!!ms-fresh :x86-operand-from-modr/m-and-sib-bytes flg0))
@@ -118,13 +129,25 @@
         (!!ms-fresh :instruction-length addr-diff))
 
        ;; Update the x86 state:
+       (x86 (!rip temp-rip x86))
        (zf (if (int= reg/mem 0) 1 0))
        (x86 (!flgi #.*zf* zf x86))
+       ;; [Shilpi:] CF, OF, SF, AF, PF are always undefined.
+       (x86 (!flgi-undefined #.*cf* x86))
+       (x86 (!flgi-undefined #.*of* x86))
+       (x86 (!flgi-undefined #.*sf* x86))
+       (x86 (!flgi-undefined #.*af* x86))
+       (x86 (!flgi-undefined #.*pf* x86))
 
-       (x86 (!rip temp-rip x86))
-
+       ;; [Shilpi:] DEST (register rgf-index) should be undefined if
+       ;; reg/mem = 0.
        ((when (int= reg/mem 0))
-        x86)
+        (b* (((mv val x86)
+              (pop-x86-oracle x86))
+             (x86 (!rgfi-size operand-size rgf-index
+                              (loghead (ash operand-size 3) (nfix val))
+                              rex-byte x86)))
+            x86))
 
        (index (the (unsigned-byte 6) (bsf 0 reg/mem)))
        (x86 (!rgfi-size operand-size rgf-index index rex-byte x86)))
