books/projects/x86isa/machine/instructions/fp/x86-fp-arithmetic-instructions.lisp
@@ -20,75 +20,24 @@
 (def-inst x86-adds?/subs?/muls?/divs?/maxs?/mins?-Op/En-RM
 
   :parents (two-byte-opcodes fp-opcodes)
-  :implemented
-  (progn
-    (add-to-implemented-opcodes-table 'ADDSS #x0F58
-				      '(:misc
-					(eql #.*mandatory-f3h* (prefixes-slice :group-1-prefix prefixes)))
-				      'x86-adds?/subs?/muls?/divs?/maxs?/mins?-Op/En-RM)
-    (add-to-implemented-opcodes-table 'SUBSS #x0F5C
-				      '(:misc
-					(eql #.*mandatory-f3h* (prefixes-slice :group-1-prefix prefixes)))
-				      'x86-adds?/subs?/muls?/divs?/maxs?/mins?-Op/En-RM)
-    (add-to-implemented-opcodes-table 'MULSS #x0F59
-				      '(:misc
-					(eql #.*mandatory-f3h* (prefixes-slice :group-1-prefix prefixes)))
-				      'x86-adds?/subs?/muls?/divs?/maxs?/mins?-Op/En-RM)
-    (add-to-implemented-opcodes-table 'DIVSS #x0F5E
-				      '(:misc
-					(eql #.*mandatory-f3h* (prefixes-slice :group-1-prefix prefixes)))
-				      'x86-adds?/subs?/muls?/divs?/maxs?/mins?-Op/En-RM)
-    (add-to-implemented-opcodes-table 'MAXSS #x0F5F
-				      '(:misc
-					(eql #.*mandatory-f3h* (prefixes-slice :group-1-prefix prefixes)))
-				      'x86-adds?/subs?/muls?/divs?/maxs?/mins?-Op/En-RM)
-    (add-to-implemented-opcodes-table 'MINSS #x0F5D
-				      '(:misc
-					(eql #.*mandatory-f3h* (prefixes-slice :group-1-prefix prefixes)))
-				      'x86-adds?/subs?/muls?/divs?/maxs?/mins?-Op/En-RM)
-
-    (add-to-implemented-opcodes-table 'ADDSD #x0F58
-				      '(:misc
-					(eql #.*mandatory-f2h* (prefixes-slice :group-1-prefix prefixes)))
-				      'x86-adds?/subs?/muls?/divs?/maxs?/mins?-Op/En-RM)
-    (add-to-implemented-opcodes-table 'SUBSD #x0F5C
-				      '(:misc
-					(eql #.*mandatory-f2h* (prefixes-slice :group-1-prefix prefixes)))
-				      'x86-adds?/subs?/muls?/divs?/maxs?/mins?-Op/En-RM)
-    (add-to-implemented-opcodes-table 'MULSD #x0F59
-				      '(:misc
-					(eql #.*mandatory-f2h* (prefixes-slice :group-1-prefix prefixes)))
-				      'x86-adds?/subs?/muls?/divs?/maxs?/mins?-Op/En-RM)
-    (add-to-implemented-opcodes-table 'DIVSD #x0F5E
-				      '(:misc
-					(eql #.*mandatory-f2h* (prefixes-slice :group-1-prefix prefixes)))
-				      'x86-adds?/subs?/muls?/divs?/maxs?/mins?-Op/En-RM)
-    (add-to-implemented-opcodes-table 'MAXSD #x0F5F
-				      '(:misc
-					(eql #.*mandatory-f2h* (prefixes-slice :group-1-prefix prefixes)))
-				      'x86-adds?/subs?/muls?/divs?/maxs?/mins?-Op/En-RM)
-    (add-to-implemented-opcodes-table 'MINSD #x0F5D
-				      '(:misc
-					(eql #.*mandatory-f2h* (prefixes-slice :group-1-prefix prefixes)))
-				      'x86-adds?/subs?/muls?/divs?/maxs?/mins?-Op/En-RM))
 
   :short "Add/Sub/Mul/Div/Max/Min scalar single/double precision floating-point values"
 
   :long
   "<h3>Op/En = RM: \[OP XMM, XMM/M\]</h3>
   F3 0F 58: ADDSS xmm1, xmm2/m32<br/>
-  F3 0F 5C: SUBSS xmm1, xmm2/m32<br/>
   F3 0F 59: MULSS xmm1, xmm2/m32<br/>
+  F3 0F 5C: SUBSS xmm1, xmm2/m32<br/>
+  F3 0F 5D: MINSS xmm1, xmm2/m32<br/>
   F3 0F 5E: DIVSS xmm1, xmm2/m32<br/>
   F3 0F 5F: MAXSS xmm1, xmm2/m32<br/>
-  F3 0F 5D: MINSS xmm1, xmm2/m32<br/>
 
   F2 0F 58: ADDSD xmm1, xmm2/m64<br/>
-  F2 0F 5C: SUBSD xmm1, xmm2/m64<br/>
   F2 0F 59: MULSD xmm1, xmm2/m64<br/>
+  F2 0F 5C: SUBSD xmm1, xmm2/m64<br/>
+  F2 0F 5D: MINSD xmm1, xmm2/m64<br/>
   F2 0F 5E: DIVSD xmm1, xmm2/m64<br/>
-  F2 0F 5F: MAXSD xmm1, xmm2/m64<br/>
-  F2 0F 5D: MINSD xmm1, xmm2/m64<br/>"
+  F2 0F 5F: MAXSD xmm1, xmm2/m64<br/>"
 
   :operation t
 
@@ -101,61 +50,57 @@
        (r/m (the (unsigned-byte 3) (mrm-r/m  modr/m)))
        (mod (the (unsigned-byte 2) (mrm-mod  modr/m)))
        (reg (the (unsigned-byte 3) (mrm-reg  modr/m)))
-       (lock (eql #.*lock*
-		  (prefixes-slice :group-1-prefix prefixes)))
+       (lock (eql #.*lock* (prefixes-slice :group-1-prefix prefixes)))
        ((when lock)
-	(!!ms-fresh :lock-prefix prefixes))
+        (!!ms-fresh :lock-prefix prefixes))
 
        ((the (integer 4 8) operand-size)
-	(if (equal sp/dp #.*OP-DP*) 8 4))
+        (if (equal sp/dp #.*OP-DP*) 8 4))
 
        ((the (unsigned-byte 4) xmm-index)
-	(reg-index reg rex-byte #.*r*))
+        (reg-index reg rex-byte #.*r*))
 
-       (xmm
-	(xmmi-size operand-size xmm-index x86))
+       (xmm (xmmi-size operand-size xmm-index x86))
 
        (p2 (prefixes-slice :group-2-prefix prefixes))
 
-       (p4? (eql #.*addr-size-override*
-		 (prefixes-slice :group-4-prefix prefixes)))
+       (p4? (eql #.*addr-size-override* (prefixes-slice :group-4-prefix prefixes)))
 
        ((mv flg0 xmm/mem (the (integer 0 4) increment-RIP-by) (the (signed-byte 64) ?v-addr) x86)
-	(x86-operand-from-modr/m-and-sib-bytes #.*xmm-access* operand-size
-					       p2 p4? temp-rip
-					       rex-byte r/m mod sib 0 x86))
+        (x86-operand-from-modr/m-and-sib-bytes
+         #.*xmm-access* operand-size p2 p4? temp-rip rex-byte r/m mod sib 0 x86))
 
        ((when flg0)
-	(!!ms-fresh :x86-operand-from-modr/m-and-sib-bytes flg0))
+        (!!ms-fresh :x86-operand-from-modr/m-and-sib-bytes flg0))
 
        ((the (signed-byte #.*max-linear-address-size+1*) temp-rip)
-	(+ temp-rip increment-RIP-by))
+        (+ temp-rip increment-RIP-by))
 
        ((when (mbe :logic (not (canonical-address-p temp-rip))
-		   :exec (<= #.*2^47*
-			     (the (signed-byte
-				   #.*max-linear-address-size+1*)
-			       temp-rip))))
-	(!!ms-fresh :temp-rip-not-canonical temp-rip))
+                   :exec (<= #.*2^47*
+                             (the (signed-byte
+                                   #.*max-linear-address-size+1*)
+                               temp-rip))))
+        (!!ms-fresh :temp-rip-not-canonical temp-rip))
 
        ((the (signed-byte #.*max-linear-address-size+1*) addr-diff)
-	(-
-	 (the (signed-byte #.*max-linear-address-size*)
-	   temp-rip)
-	 (the (signed-byte #.*max-linear-address-size*)
-	   start-rip)))
+        (-
+         (the (signed-byte #.*max-linear-address-size*)
+           temp-rip)
+         (the (signed-byte #.*max-linear-address-size*)
+           start-rip)))
        ((when (< 15 addr-diff))
-	(!!ms-fresh :instruction-length addr-diff))
+        (!!ms-fresh :instruction-length addr-diff))
 
        ((mv flg1 result (the (unsigned-byte 32) mxcsr))
-	(if (equal sp/dp #.*OP-DP*)
-	    (dp-sse-add/sub/mul/div/max/min operation xmm xmm/mem (mxcsr x86))
-	  (sp-sse-add/sub/mul/div/max/min operation xmm xmm/mem (mxcsr x86))))
+        (if (equal sp/dp #.*OP-DP*)
+            (dp-sse-add/sub/mul/div/max/min operation xmm xmm/mem (mxcsr x86))
+          (sp-sse-add/sub/mul/div/max/min operation xmm xmm/mem (mxcsr x86))))
 
        ((when flg1)
-	(if (equal sp/dp #.*OP-DP*)
-	    (!!ms-fresh :dp-sse-add/sub/mul/div/max/min flg1)
-	  (!!ms-fresh :sp-sse-add/sub/mul/div/max/min flg1)))
+        (if (equal sp/dp #.*OP-DP*)
+            (!!ms-fresh :dp-sse-add/sub/mul/div/max/min flg1)
+          (!!ms-fresh :sp-sse-add/sub/mul/div/max/min flg1)))
 
        ;; Update the x86 state:
        (x86 (!mxcsr mxcsr x86))
@@ -163,31 +108,52 @@
        (x86 (!xmmi-size operand-size xmm-index result x86))
 
        (x86 (!rip temp-rip x86)))
-      x86))
+      x86)
+
+  :implemented
+  (progn
+    (add-to-implemented-opcodes-table 'ADDSS #x0F58
+                                      '(:misc
+                                        (eql #.*mandatory-f3h* (prefixes-slice :group-1-prefix prefixes)))
+                                      'x86-adds?/subs?/muls?/divs?/maxs?/mins?-Op/En-RM)
+    (add-to-implemented-opcodes-table 'MULSS #x0F59
+                                      '(:misc (eql #.*mandatory-f3h* (prefixes-slice :group-1-prefix prefixes)))
+                                      'x86-adds?/subs?/muls?/divs?/maxs?/mins?-Op/En-RM)
+    (add-to-implemented-opcodes-table 'SUBSS #x0F5C
+                                      '(:misc (eql #.*mandatory-f3h* (prefixes-slice :group-1-prefix prefixes)))
+                                      'x86-adds?/subs?/muls?/divs?/maxs?/mins?-Op/En-RM)
+    (add-to-implemented-opcodes-table 'MINSS #x0F5D
+                                      '(:misc (eql #.*mandatory-f3h* (prefixes-slice :group-1-prefix prefixes)))
+                                      'x86-adds?/subs?/muls?/divs?/maxs?/mins?-Op/En-RM)
+    (add-to-implemented-opcodes-table 'DIVSS #x0F5E
+                                      '(:misc (eql #.*mandatory-f3h* (prefixes-slice :group-1-prefix prefixes)))
+                                      'x86-adds?/subs?/muls?/divs?/maxs?/mins?-Op/En-RM)
+    (add-to-implemented-opcodes-table 'MAXSS #x0F5F
+                                      '(:misc (eql #.*mandatory-f3h* (prefixes-slice :group-1-prefix prefixes)))
+                                      'x86-adds?/subs?/muls?/divs?/maxs?/mins?-Op/En-RM)
+
+    (add-to-implemented-opcodes-table 'ADDSD #x0F58
+                                      '(:misc (eql #.*mandatory-f2h* (prefixes-slice :group-1-prefix prefixes)))
+                                      'x86-adds?/subs?/muls?/divs?/maxs?/mins?-Op/En-RM)
+    (add-to-implemented-opcodes-table 'MULSD #x0F59
+                                      '(:misc (eql #.*mandatory-f2h* (prefixes-slice :group-1-prefix prefixes)))
+                                      'x86-adds?/subs?/muls?/divs?/maxs?/mins?-Op/En-RM)
+    (add-to-implemented-opcodes-table 'SUBSD #x0F5C
+                                      '(:misc (eql #.*mandatory-f2h* (prefixes-slice :group-1-prefix prefixes)))
+                                      'x86-adds?/subs?/muls?/divs?/maxs?/mins?-Op/En-RM)
+    (add-to-implemented-opcodes-table 'MINSD #x0F5D
+                                      '(:misc (eql #.*mandatory-f2h* (prefixes-slice :group-1-prefix prefixes)))
+                                      'x86-adds?/subs?/muls?/divs?/maxs?/mins?-Op/En-RM)
+    (add-to-implemented-opcodes-table 'DIVSD #x0F5E
+                                      '(:misc (eql #.*mandatory-f2h* (prefixes-slice :group-1-prefix prefixes)))
+                                      'x86-adds?/subs?/muls?/divs?/maxs?/mins?-Op/En-RM)
+    (add-to-implemented-opcodes-table 'MAXSD #x0F5F
+                                      '(:misc (eql #.*mandatory-f2h* (prefixes-slice :group-1-prefix prefixes)))
+                                      'x86-adds?/subs?/muls?/divs?/maxs?/mins?-Op/En-RM)))
 
 (def-inst x86-addps/subps/mulps/divps/maxps/minps-Op/En-RM
 
   :parents (two-byte-opcodes fp-opcodes)
-  :implemented
-  (progn
-    (add-to-implemented-opcodes-table 'ADDPS #x0F58
-                                      '(:nil nil)
-                                      'x86-addps/subps/mulps/divps/maxps/minps-Op/En-RM)
-    (add-to-implemented-opcodes-table 'SUBPS #x0F5C
-                                      '(:nil nil)
-                                      'x86-addps/subps/mulps/divps/maxps/minps-Op/En-RM)
-    (add-to-implemented-opcodes-table 'MULPS #x0F59
-                                      '(:nil nil)
-                                      'x86-addps/subps/mulps/divps/maxps/minps-Op/En-RM)
-    (add-to-implemented-opcodes-table 'DIVPS #x0F5E
-                                      '(:nil nil)
-                                      'x86-addps/subps/mulps/divps/maxps/minps-Op/En-RM)
-    (add-to-implemented-opcodes-table 'MAXPS #x0F5F
-                                      '(:nil nil)
-                                      'x86-addps/subps/mulps/divps/maxps/minps-Op/En-RM)
-    (add-to-implemented-opcodes-table 'MINPS #x0F5D
-                                      '(:nil nil)
-                                      'x86-addps/subps/mulps/divps/maxps/minps-Op/En-RM))
 
   :short "Add/Sub/Mul/Div/Max/Min packed single-precision floating-point values"
 
@@ -209,84 +175,73 @@
        (r/m (the (unsigned-byte 3) (mrm-r/m  modr/m)))
        (mod (the (unsigned-byte 2) (mrm-mod  modr/m)))
        (reg (the (unsigned-byte 3) (mrm-reg  modr/m)))
-       (lock (eql #.*lock*
-		  (prefixes-slice :group-1-prefix prefixes)))
+       (lock (eql #.*lock* (prefixes-slice :group-1-prefix prefixes)))
        ((when lock)
-	(!!ms-fresh :lock-prefix prefixes))
+        (!!ms-fresh :lock-prefix prefixes))
 
        ((the (unsigned-byte 4) xmm-index)
-	(reg-index reg rex-byte #.*r*))
+        (reg-index reg rex-byte #.*r*))
 
        ((the (unsigned-byte 128) xmm)
-	(xmmi-size 16 xmm-index x86))
+        (xmmi-size 16 xmm-index x86))
 
        (p2 (prefixes-slice :group-2-prefix prefixes))
 
-       (p4? (eql #.*addr-size-override*
-		 (prefixes-slice :group-4-prefix prefixes)))
+       (p4? (eql #.*addr-size-override* (prefixes-slice :group-4-prefix prefixes)))
 
        ((mv flg0
             (the (unsigned-byte 128) xmm/mem)
             (the (integer 0 4) increment-RIP-by)
             (the (signed-byte 64) ?v-addr) x86)
-	(x86-operand-from-modr/m-and-sib-bytes #.*xmm-access* 16
-					       p2 p4? temp-rip
-					       rex-byte r/m mod sib 0 x86))
+        (x86-operand-from-modr/m-and-sib-bytes
+         #.*xmm-access* 16 p2 p4? temp-rip rex-byte r/m mod sib 0 x86))
 
        ((when flg0)
-	(!!ms-fresh :x86-operand-from-modr/m-and-sib-bytes flg0))
+        (!!ms-fresh :x86-operand-from-modr/m-and-sib-bytes flg0))
 
        ((the (signed-byte #.*max-linear-address-size+1*) temp-rip)
-	(+ temp-rip increment-RIP-by))
+        (+ temp-rip increment-RIP-by))
 
        ((when (mbe :logic (not (canonical-address-p temp-rip))
-		   :exec (<= #.*2^47*
-			     (the (signed-byte
-				   #.*max-linear-address-size+1*)
-			       temp-rip))))
-	(!!ms-fresh :temp-rip-not-canonical temp-rip))
+                   :exec (<= #.*2^47*
+                             (the (signed-byte
+                                   #.*max-linear-address-size+1*)
+                               temp-rip))))
+        (!!ms-fresh :temp-rip-not-canonical temp-rip))
 
        ((the (signed-byte #.*max-linear-address-size+1*) addr-diff)
-	(-
-	 (the (signed-byte #.*max-linear-address-size*)
-	   temp-rip)
-	 (the (signed-byte #.*max-linear-address-size*)
-	   start-rip)))
+        (-
+         (the (signed-byte #.*max-linear-address-size*)
+           temp-rip)
+         (the (signed-byte #.*max-linear-address-size*)
+           start-rip)))
        ((when (< 15 addr-diff))
-	(!!ms-fresh :instruction-length addr-diff))
+        (!!ms-fresh :instruction-length addr-diff))
 
-       ;; Raise an error if v-addr is not 16-byte aligned. 
+       ;; Raise an error if v-addr is not 16-byte aligned.
        ;; In case the second operand is an XMM register, v-addr = 0.
        ((when (not (eql (mod v-addr 16) 0)))
         (!!ms-fresh :memory-address-is-not-16-byte-aligned v-addr))
 
        (xmm0 (mbe :logic (part-select xmm :low 0 :high 31)
-                  :exec  (the (unsigned-byte 32)
-                              (logand #uxFFFF_FFFF xmm))))
+                  :exec  (the (unsigned-byte 32) (logand #uxFFFF_FFFF xmm))))
        (xmm/mem0 (mbe :logic (part-select xmm/mem :low 0 :high 31)
-                      :exec  (the (unsigned-byte 32)
-                                  (logand #uxFFFF_FFFF xmm/mem))))
+                      :exec  (the (unsigned-byte 32) (logand #uxFFFF_FFFF xmm/mem))))
 
        (xmm1 (mbe :logic (part-select xmm :low 32 :high 63)
-                  :exec  (the (unsigned-byte 32)
-                              (logand #uxFFFF_FFFF (ash xmm -32)))))
+                  :exec  (the (unsigned-byte 32) (logand #uxFFFF_FFFF (ash xmm -32)))))
        (xmm/mem1 (mbe :logic (part-select xmm/mem :low 32 :high 63)
-                      :exec  (the (unsigned-byte 32)
-                                  (logand #uxFFFF_FFFF (ash xmm/mem -32)))))
+                      :exec  (the (unsigned-byte 32) (logand #uxFFFF_FFFF (ash xmm/mem -32)))))
 
        (xmm2 (mbe :logic (part-select xmm :low 64 :high 95)
-                  :exec  (the (unsigned-byte 32)
-                              (logand #uxFFFF_FFFF (ash xmm -64)))))
+                  :exec  (the (unsigned-byte 32) (logand #uxFFFF_FFFF (ash xmm -64)))))
        (xmm/mem2 (mbe :logic (part-select xmm/mem :low 64 :high 95)
-                      :exec  (the (unsigned-byte 32)
-                                  (logand #uxFFFF_FFFF (ash xmm/mem -64)))))
+                      :exec  (the (unsigned-byte 32) (logand #uxFFFF_FFFF (ash xmm/mem -64)))))
 
        (xmm3 (mbe :logic (part-select xmm :low 96 :high 127)
-                  :exec  (the (unsigned-byte 32)
-                              (logand #uxFFFF_FFFF (ash xmm -96)))))
+                  :exec  (the (unsigned-byte 32) (logand #uxFFFF_FFFF (ash xmm -96)))))
        (xmm/mem3 (mbe :logic (part-select xmm/mem :low 96 :high 127)
-                      :exec  (the (unsigned-byte 32)
-                                  (logand #uxFFFF_FFFF (ash xmm/mem -96)))))
+                      :exec  (the (unsigned-byte 32) (logand #uxFFFF_FFFF (ash xmm/mem -96)))))
 
        (mxcsr (the (unsigned-byte 32) (mxcsr x86)))
 
@@ -325,7 +280,7 @@
        (result (merge-4-u32s result3 result2 result1 result0))
 
        (mxcsr (the (unsigned-byte 32)
-                   (logior mxcsr0 mxcsr1 mxcsr2 mxcsr3)))
+                (logior mxcsr0 mxcsr1 mxcsr2 mxcsr3)))
 
        ;; Update the x86 state:
        (x86 (!mxcsr mxcsr x86))
@@ -333,48 +288,43 @@
        (x86 (!xmmi-size 16 xmm-index result x86))
 
        (x86 (!rip temp-rip x86)))
-      x86))
+      x86)
+
+  :implemented
+  (progn
+    (add-to-implemented-opcodes-table 'ADDPS #x0F58
+                                      '(:nil nil)
+                                      'x86-addps/subps/mulps/divps/maxps/minps-Op/En-RM)
+    (add-to-implemented-opcodes-table 'MULPS #x0F59
+                                      '(:nil nil)
+                                      'x86-addps/subps/mulps/divps/maxps/minps-Op/En-RM)
+    (add-to-implemented-opcodes-table 'SUBPS #x0F5C
+                                      '(:nil nil)
+                                      'x86-addps/subps/mulps/divps/maxps/minps-Op/En-RM)
+    (add-to-implemented-opcodes-table 'MINPS #x0F5D
+                                      '(:nil nil)
+                                      'x86-addps/subps/mulps/divps/maxps/minps-Op/En-RM)
+    (add-to-implemented-opcodes-table 'DIVPS #x0F5E
+                                      '(:nil nil)
+                                      'x86-addps/subps/mulps/divps/maxps/minps-Op/En-RM)
+    (add-to-implemented-opcodes-table 'MAXPS #x0F5F
+                                      '(:nil nil)
+                                      'x86-addps/subps/mulps/divps/maxps/minps-Op/En-RM)))
 
 (def-inst x86-addpd/subpd/mulpd/divpd/maxpd/minpd-Op/En-RM
 
   :parents (two-byte-opcodes fp-opcodes)
-  :implemented
-  (progn
-    (add-to-implemented-opcodes-table 'ADDPD #x0F58
-                                      '(:misc
-					(eql #.*mandatory-66h* (prefixes-slice :group-3-prefix prefixes)))
-                                      'x86-addpd/subpd/mulpd/divpd/maxpd/minpd-Op/En-RM)
-    (add-to-implemented-opcodes-table 'SUBPD #x0F5C
-                                      '(:misc
-					(eql #.*mandatory-66h* (prefixes-slice :group-3-prefix prefixes)))
-                                      'x86-addpd/subpd/mulpd/divpd/maxpd/minpd-Op/En-RM)
-    (add-to-implemented-opcodes-table 'MULPD #x0F59
-                                      '(:misc
-					(eql #.*mandatory-66h* (prefixes-slice :group-3-prefix prefixes)))
-                                      'x86-addpd/subpd/mulpd/divpd/maxpd/minpd-Op/En-RM)
-    (add-to-implemented-opcodes-table 'DIVPD #x0F5E
-                                      '(:misc
-					(eql #.*mandatory-66h* (prefixes-slice :group-3-prefix prefixes)))
-                                      'x86-addpd/subpd/mulpd/divpd/maxpd/minpd-Op/En-RM)
-    (add-to-implemented-opcodes-table 'MAXPD #x0F5F
-                                      '(:misc
-					(eql #.*mandatory-66h* (prefixes-slice :group-3-prefix prefixes)))
-                                      'x86-addpd/subpd/mulpd/divpd/maxpd/minpd-Op/En-RM)
-    (add-to-implemented-opcodes-table 'MINPD #x0F5D
-                                      '(:misc
-					(eql #.*mandatory-66h* (prefixes-slice :group-3-prefix prefixes)))
-                                      'x86-addpd/subpd/mulpd/divpd/maxpd/minpd-Op/En-RM))
 
   :short "Add/Sub/Mul/Div/Max/Min packed double-precision floating-point values"
 
   :long
   "<h3>Op/En = RM: \[OP XMM, XMM/M\]</h3>
   66 0F 58: ADDPD xmm1, xmm2/m128<br/>
-  66 0F 5C: SUBPD xmm1, xmm2/m128<br/>
   66 0F 59: MULPD xmm1, xmm2/m128<br/>
+  66 0F 5C: SUBPD xmm1, xmm2/m128<br/>
+  66 0F 5D: MINPD xmm1, xmm2/m128<br/>
   66 0F 5E: DIVPD xmm1, xmm2/m128<br/>
-  66 0F 5F: MAXPD xmm1, xmm2/m128<br/>
-  66 0F 5D: MINPD xmm1, xmm2/m128<br/>"
+  66 0F 5F: MAXPD xmm1, xmm2/m128<br/>"
 
   :operation t
 
@@ -385,70 +335,67 @@
        (r/m (the (unsigned-byte 3) (mrm-r/m  modr/m)))
        (mod (the (unsigned-byte 2) (mrm-mod  modr/m)))
        (reg (the (unsigned-byte 3) (mrm-reg  modr/m)))
-       (lock (eql #.*lock*
-		  (prefixes-slice :group-1-prefix prefixes)))
+       (lock (eql #.*lock* (prefixes-slice :group-1-prefix prefixes)))
        ((when lock)
-	(!!ms-fresh :lock-prefix prefixes))
+        (!!ms-fresh :lock-prefix prefixes))
 
        ((the (unsigned-byte 4) xmm-index)
-	(reg-index reg rex-byte #.*r*))
+        (reg-index reg rex-byte #.*r*))
 
        ((the (unsigned-byte 128) xmm)
-	(xmmi-size 16 xmm-index x86))
+        (xmmi-size 16 xmm-index x86))
 
        (p2 (prefixes-slice :group-2-prefix prefixes))
 
-       (p4? (eql #.*addr-size-override*
-		 (prefixes-slice :group-4-prefix prefixes)))
+       (p4? (eql #.*addr-size-override* (prefixes-slice :group-4-prefix prefixes)))
 
        ((mv flg0
             (the (unsigned-byte 128) xmm/mem)
             (the (integer 0 4) increment-RIP-by)
             (the (signed-byte 64) ?v-addr) x86)
-	(x86-operand-from-modr/m-and-sib-bytes #.*xmm-access* 16
-					       p2 p4? temp-rip
-					       rex-byte r/m mod sib 0 x86))
+        (x86-operand-from-modr/m-and-sib-bytes
+         #.*xmm-access* 16 p2 p4? temp-rip rex-byte r/m mod sib 0 x86))
 
        ((when flg0)
-	(!!ms-fresh :x86-operand-from-modr/m-and-sib-bytes flg0))
+        (!!ms-fresh :x86-operand-from-modr/m-and-sib-bytes flg0))
 
        ((the (signed-byte #.*max-linear-address-size+1*) temp-rip)
-	(+ temp-rip increment-RIP-by))
+        (+ temp-rip increment-RIP-by))
 
        ((when (mbe :logic (not (canonical-address-p temp-rip))
-		   :exec (<= #.*2^47*
-			     (the (signed-byte
-				   #.*max-linear-address-size+1*)
-			       temp-rip))))
-	(!!ms-fresh :temp-rip-not-canonical temp-rip))
+                   :exec (<= #.*2^47*
+                             (the (signed-byte
+                                   #.*max-linear-address-size+1*)
+                               temp-rip))))
+        (!!ms-fresh :temp-rip-not-canonical temp-rip))
 
        ((the (signed-byte #.*max-linear-address-size+1*) addr-diff)
-	(-
-	 (the (signed-byte #.*max-linear-address-size*)
-	   temp-rip)
-	 (the (signed-byte #.*max-linear-address-size*)
-	   start-rip)))
+        (-
+         (the (signed-byte #.*max-linear-address-size*)
+           temp-rip)
+         (the (signed-byte #.*max-linear-address-size*)
+           start-rip)))
        ((when (< 15 addr-diff))
-	(!!ms-fresh :instruction-length addr-diff))
+        (!!ms-fresh :instruction-length addr-diff))
 
-       ;; Raise an error if v-addr is not 16-byte aligned. 
+       ;; Raise an error if v-addr is not 16-byte aligned.
        ;; In case the second operand is an XMM register, v-addr = 0.
        ((when (not (eql (mod v-addr 16) 0)))
         (!!ms-fresh :memory-address-is-not-16-byte-aligned v-addr))
 
        (xmm0 (mbe :logic (part-select xmm :low 0 :high 63)
                   :exec  (the (unsigned-byte 64)
-                              (logand #uxFFFF_FFFF_FFFF_FFFF xmm))))
+                           (logand #uxFFFF_FFFF_FFFF_FFFF xmm))))
        (xmm/mem0 (mbe :logic (part-select xmm/mem :low 0 :high 63)
                       :exec  (the (unsigned-byte 64)
-                                  (logand #uxFFFF_FFFF_FFFF_FFFF xmm/mem))))
+                               (logand #uxFFFF_FFFF_FFFF_FFFF xmm/mem))))
 
        (xmm1 (mbe :logic (part-select xmm :low 64 :high 127)
                   :exec  (the (unsigned-byte 64)
-                              (logand #uxFFFF_FFFF_FFFF_FFFF (ash xmm -64)))))
+                           (logand #uxFFFF_FFFF_FFFF_FFFF (ash xmm -64)))))
        (xmm/mem1 (mbe :logic (part-select xmm/mem :low 64 :high 127)
                       :exec  (the (unsigned-byte 64)
-                                  (logand #uxFFFF_FFFF_FFFF_FFFF (ash xmm/mem -64)))))
+                               (logand #uxFFFF_FFFF_FFFF_FFFF (ash xmm/mem -64)))))
 
        (mxcsr (the (unsigned-byte 32) (mxcsr x86)))
 
@@ -471,7 +418,7 @@
        (result (merge-2-u64s result1 result0))
 
        (mxcsr (the (unsigned-byte 32)
-                   (logior mxcsr0 mxcsr1)))
+                (logior mxcsr0 mxcsr1)))
 
        ;; Update the x86 state:
        (x86 (!mxcsr mxcsr x86))
@@ -479,21 +426,38 @@
        (x86 (!xmmi-size 16 xmm-index result x86))
 
        (x86 (!rip temp-rip x86)))
-      x86))
+      x86)
+
+  :implemented
+  (progn
+    (add-to-implemented-opcodes-table 'ADDPD #x0F58
+                                      '(:misc
+                                        (eql #.*mandatory-66h* (prefixes-slice :group-3-prefix prefixes)))
+                                      'x86-addpd/subpd/mulpd/divpd/maxpd/minpd-Op/En-RM)
+    (add-to-implemented-opcodes-table 'SUBPD #x0F5C
+                                      '(:misc
+                                        (eql #.*mandatory-66h* (prefixes-slice :group-3-prefix prefixes)))
+                                      'x86-addpd/subpd/mulpd/divpd/maxpd/minpd-Op/En-RM)
+    (add-to-implemented-opcodes-table 'MULPD #x0F59
+                                      '(:misc
+                                        (eql #.*mandatory-66h* (prefixes-slice :group-3-prefix prefixes)))
+                                      'x86-addpd/subpd/mulpd/divpd/maxpd/minpd-Op/En-RM)
+    (add-to-implemented-opcodes-table 'DIVPD #x0F5E
+                                      '(:misc
+                                        (eql #.*mandatory-66h* (prefixes-slice :group-3-prefix prefixes)))
+                                      'x86-addpd/subpd/mulpd/divpd/maxpd/minpd-Op/En-RM)
+    (add-to-implemented-opcodes-table 'MAXPD #x0F5F
+                                      '(:misc
+                                        (eql #.*mandatory-66h* (prefixes-slice :group-3-prefix prefixes)))
+                                      'x86-addpd/subpd/mulpd/divpd/maxpd/minpd-Op/En-RM)
+    (add-to-implemented-opcodes-table 'MINPD #x0F5D
+                                      '(:misc
+                                        (eql #.*mandatory-66h* (prefixes-slice :group-3-prefix prefixes)))
+                                      'x86-addpd/subpd/mulpd/divpd/maxpd/minpd-Op/En-RM)))
 
 (def-inst x86-sqrts?-Op/En-RM
 
   :parents (two-byte-opcodes fp-opcodes)
-  :implemented
-  (progn
-    (add-to-implemented-opcodes-table 'SQRTSS #x0F51
-				      '(:misc
-					(eql #.*mandatory-f3h* (prefixes-slice :group-1-prefix prefixes)))
-				      'x86-sqrts?-Op/En-RM)
-    (add-to-implemented-opcodes-table 'SQRTSD #x0F51
-				      '(:misc
-					(eql #.*mandatory-f2h* (prefixes-slice :group-1-prefix prefixes)))
-				      'x86-sqrts?-Op/En-RM))
 
   :short "Square root of scalar single/double precision floating-point value"
 
@@ -511,58 +475,55 @@
        (r/m (the (unsigned-byte 3) (mrm-r/m  modr/m)))
        (mod (the (unsigned-byte 2) (mrm-mod  modr/m)))
        (reg (the (unsigned-byte 3) (mrm-reg  modr/m)))
-       (lock (eql #.*lock*
-		  (prefixes-slice :group-1-prefix prefixes)))
+       (lock (eql #.*lock* (prefixes-slice :group-1-prefix prefixes)))
        ((when lock)
-	(!!ms-fresh :lock-prefix prefixes))
+        (!!ms-fresh :lock-prefix prefixes))
 
        ((the (integer 4 8) operand-size)
-	(if (equal sp/dp #.*OP-DP*) 8 4))
+        (if (equal sp/dp #.*OP-DP*) 8 4))
 
        ((the (unsigned-byte 4) xmm-index)
-	(reg-index reg rex-byte #.*r*))
+        (reg-index reg rex-byte #.*r*))
 
        (p2 (prefixes-slice :group-2-prefix prefixes))
 
-       (p4? (eql #.*addr-size-override*
-		 (prefixes-slice :group-4-prefix prefixes)))
+       (p4? (eql #.*addr-size-override* (prefixes-slice :group-4-prefix prefixes)))
 
        ((mv flg0 xmm/mem (the (integer 0 4) increment-RIP-by) (the (signed-byte 64) ?v-addr) x86)
-	(x86-operand-from-modr/m-and-sib-bytes #.*xmm-access* operand-size
-					       p2 p4? temp-rip
-					       rex-byte r/m mod sib 0 x86))
+        (x86-operand-from-modr/m-and-sib-bytes
+         #.*xmm-access* operand-size p2 p4? temp-rip rex-byte r/m mod sib 0 x86))
 
        ((when flg0)
-	(!!ms-fresh :x86-operand-from-modr/m-and-sib-bytes flg0))
+        (!!ms-fresh :x86-operand-from-modr/m-and-sib-bytes flg0))
 
        ((the (signed-byte #.*max-linear-address-size+1*) temp-rip)
-	(+ temp-rip increment-RIP-by))
+        (+ temp-rip increment-RIP-by))
 
        ((when (mbe :logic (not (canonical-address-p temp-rip))
-		   :exec (<= #.*2^47*
-			     (the (signed-byte
-				   #.*max-linear-address-size+1*)
-			       temp-rip))))
-	(!!ms-fresh :temp-rip-not-canonical temp-rip))
+                   :exec (<= #.*2^47*
+                             (the (signed-byte
+                                   #.*max-linear-address-size+1*)
+                               temp-rip))))
+        (!!ms-fresh :temp-rip-not-canonical temp-rip))
 
        ((the (signed-byte #.*max-linear-address-size+1*) addr-diff)
-	(-
-	 (the (signed-byte #.*max-linear-address-size*)
-	   temp-rip)
-	 (the (signed-byte #.*max-linear-address-size*)
-	   start-rip)))
+        (-
+         (the (signed-byte #.*max-linear-address-size*)
+           temp-rip)
+         (the (signed-byte #.*max-linear-address-size*)
+           start-rip)))
        ((when (< 15 addr-diff))
-	(!!ms-fresh :instruction-length addr-diff))
+        (!!ms-fresh :instruction-length addr-diff))
 
        ((mv flg1 result (the (unsigned-byte 32) mxcsr))
-	(if (equal sp/dp #.*OP-DP*)
-	    (dp-sse-sqrt xmm/mem (mxcsr x86))
-	  (sp-sse-sqrt xmm/mem (mxcsr x86))))
+        (if (equal sp/dp #.*OP-DP*)
+            (dp-sse-sqrt xmm/mem (mxcsr x86))
+          (sp-sse-sqrt xmm/mem (mxcsr x86))))
 
        ((when flg1)
-	(if (equal sp/dp #.*OP-DP*)
-	    (!!ms-fresh :dp-sse-sqrt flg1)
-	  (!!ms-fresh :sp-sse-sqrt flg1)))
+        (if (equal sp/dp #.*OP-DP*)
+            (!!ms-fresh :dp-sse-sqrt flg1)
+          (!!ms-fresh :sp-sse-sqrt flg1)))
 
        ;; Update the x86 state:
        (x86 (!mxcsr mxcsr x86))
@@ -570,15 +531,22 @@
        (x86 (!xmmi-size operand-size xmm-index result x86))
 
        (x86 (!rip temp-rip x86)))
-      x86))
+      x86)
+
+  :implemented
+  (progn
+    (add-to-implemented-opcodes-table 'SQRTSS #x0F51
+                                      '(:misc
+                                        (eql #.*mandatory-f3h* (prefixes-slice :group-1-prefix prefixes)))
+                                      'x86-sqrts?-Op/En-RM)
+    (add-to-implemented-opcodes-table 'SQRTSD #x0F51
+                                      '(:misc
+                                        (eql #.*mandatory-f2h* (prefixes-slice :group-1-prefix prefixes)))
+                                      'x86-sqrts?-Op/En-RM)))
 
 (def-inst x86-sqrtps-Op/En-RM
 
   :parents (two-byte-opcodes fp-opcodes)
-  :implemented
-  (add-to-implemented-opcodes-table 'SQRTPS #x0F51
-                                    '(:nil nil)
-                                    'x86-sqrtps-Op/En-RM)
 
   :short "Square roots of packed single-precision floating-point values"
 
@@ -593,69 +561,66 @@
        (r/m (the (unsigned-byte 3) (mrm-r/m  modr/m)))
        (mod (the (unsigned-byte 2) (mrm-mod  modr/m)))
        (reg (the (unsigned-byte 3) (mrm-reg  modr/m)))
-       (lock (eql #.*lock*
-		  (prefixes-slice :group-1-prefix prefixes)))
+       (lock (eql #.*lock* (prefixes-slice :group-1-prefix prefixes)))
        ((when lock)
-	(!!ms-fresh :lock-prefix prefixes))
+        (!!ms-fresh :lock-prefix prefixes))
 
        ((the (unsigned-byte 4) xmm-index)
-	(reg-index reg rex-byte #.*r*))
+        (reg-index reg rex-byte #.*r*))
 
        (p2 (prefixes-slice :group-2-prefix prefixes))
 
-       (p4? (eql #.*addr-size-override*
-		 (prefixes-slice :group-4-prefix prefixes)))
+       (p4? (eql #.*addr-size-override* (prefixes-slice :group-4-prefix prefixes)))
 
        ((mv flg0
             (the (unsigned-byte 128) xmm/mem)
             (the (integer 0 4) increment-RIP-by)
             (the (signed-byte 64) ?v-addr) x86)
-	(x86-operand-from-modr/m-and-sib-bytes #.*xmm-access* 16
-					       p2 p4? temp-rip
-					       rex-byte r/m mod sib 0 x86))
+        (x86-operand-from-modr/m-and-sib-bytes
+         #.*xmm-access* 16 p2 p4? temp-rip rex-byte r/m mod sib 0 x86))
 
        ((when flg0)
-	(!!ms-fresh :x86-operand-from-modr/m-and-sib-bytes flg0))
+        (!!ms-fresh :x86-operand-from-modr/m-and-sib-bytes flg0))
 
        ((the (signed-byte #.*max-linear-address-size+1*) temp-rip)
-	(+ temp-rip increment-RIP-by))
+        (+ temp-rip increment-RIP-by))
 
        ((when (mbe :logic (not (canonical-address-p temp-rip))
-		   :exec (<= #.*2^47*
-			     (the (signed-byte
-				   #.*max-linear-address-size+1*)
-			       temp-rip))))
-	(!!ms-fresh :temp-rip-not-canonical temp-rip))
+                   :exec (<= #.*2^47*
+                             (the (signed-byte
+                                   #.*max-linear-address-size+1*)
+                               temp-rip))))
+        (!!ms-fresh :temp-rip-not-canonical temp-rip))
 
        ((the (signed-byte #.*max-linear-address-size+1*) addr-diff)
-	(-
-	 (the (signed-byte #.*max-linear-address-size*)
-	   temp-rip)
-	 (the (signed-byte #.*max-linear-address-size*)
-	   start-rip)))
+        (-
+         (the (signed-byte #.*max-linear-address-size*)
+           temp-rip)
+         (the (signed-byte #.*max-linear-address-size*)
+           start-rip)))
        ((when (< 15 addr-diff))
-	(!!ms-fresh :instruction-length addr-diff))
+        (!!ms-fresh :instruction-length addr-diff))
 
-       ;; Raise an error if v-addr is not 16-byte aligned. 
+       ;; Raise an error if v-addr is not 16-byte aligned.
        ;; In case the second operand is an XMM register, v-addr = 0.
        ((when (not (eql (mod v-addr 16) 0)))
         (!!ms-fresh :memory-address-is-not-16-byte-aligned v-addr))
 
        (xmm/mem0 (mbe :logic (part-select xmm/mem :low 0 :high 31)
                       :exec  (the (unsigned-byte 32)
-                                  (logand #uxFFFF_FFFF xmm/mem))))
+                               (logand #uxFFFF_FFFF xmm/mem))))
 
        (xmm/mem1 (mbe :logic (part-select xmm/mem :low 32 :high 63)
                       :exec  (the (unsigned-byte 32)
-                                  (logand #uxFFFF_FFFF (ash xmm/mem -32)))))
+                               (logand #uxFFFF_FFFF (ash xmm/mem -32)))))
 
        (xmm/mem2 (mbe :logic (part-select xmm/mem :low 64 :high 95)
                       :exec  (the (unsigned-byte 32)
-                                  (logand #uxFFFF_FFFF (ash xmm/mem -64)))))
+                               (logand #uxFFFF_FFFF (ash xmm/mem -64)))))
 
        (xmm/mem3 (mbe :logic (part-select xmm/mem :low 96 :high 127)
                       :exec  (the (unsigned-byte 32)
-                                  (logand #uxFFFF_FFFF (ash xmm/mem -96)))))
+                               (logand #uxFFFF_FFFF (ash xmm/mem -96)))))
 
        (mxcsr (the (unsigned-byte 32) (mxcsr x86)))
 
@@ -694,7 +659,7 @@
        (result (merge-4-u32s result3 result2 result1 result0))
 
        (mxcsr (the (unsigned-byte 32)
-                   (logior mxcsr0 mxcsr1 mxcsr2 mxcsr3)))
+                (logior mxcsr0 mxcsr1 mxcsr2 mxcsr3)))
 
        ;; Update the x86 state:
        (x86 (!mxcsr mxcsr x86))
@@ -702,16 +667,16 @@
        (x86 (!xmmi-size 16 xmm-index result x86))
 
        (x86 (!rip temp-rip x86)))
-      x86))
+      x86)
+
+  :implemented
+  (add-to-implemented-opcodes-table 'SQRTPS #x0F51
+                                    '(:nil nil)
+                                    'x86-sqrtps-Op/En-RM))
 
 (def-inst x86-sqrtpd-Op/En-RM
 
   :parents (two-byte-opcodes fp-opcodes)
-  :implemented
-  (add-to-implemented-opcodes-table 'SQRTPD #x0F51
-                                    '(:misc
-                                      (eql #.*mandatory-66h* (prefixes-slice :group-3-prefix prefixes)))
-                                    'x86-sqrtpd-Op/En-RM)
 
   :short "Square roots packed double-precision floating-point values"
 
@@ -726,61 +691,58 @@
        (r/m (the (unsigned-byte 3) (mrm-r/m  modr/m)))
        (mod (the (unsigned-byte 2) (mrm-mod  modr/m)))
        (reg (the (unsigned-byte 3) (mrm-reg  modr/m)))
-       (lock (eql #.*lock*
-		  (prefixes-slice :group-1-prefix prefixes)))
+       (lock (eql #.*lock* (prefixes-slice :group-1-prefix prefixes)))
        ((when lock)
-	(!!ms-fresh :lock-prefix prefixes))
+        (!!ms-fresh :lock-prefix prefixes))
 
        ((the (unsigned-byte 4) xmm-index)
-	(reg-index reg rex-byte #.*r*))
+        (reg-index reg rex-byte #.*r*))
 
        (p2 (prefixes-slice :group-2-prefix prefixes))
 
-       (p4? (eql #.*addr-size-override*
-		 (prefixes-slice :group-4-prefix prefixes)))
+       (p4? (eql #.*addr-size-override* (prefixes-slice :group-4-prefix prefixes)))
 
        ((mv flg0
             (the (unsigned-byte 128) xmm/mem)
             (the (integer 0 4) increment-RIP-by)
             (the (signed-byte 64) ?v-addr) x86)
-	(x86-operand-from-modr/m-and-sib-bytes #.*xmm-access* 16
-					       p2 p4? temp-rip
-					       rex-byte r/m mod sib 0 x86))
+        (x86-operand-from-modr/m-and-sib-bytes
+         #.*xmm-access* 16 p2 p4? temp-rip rex-byte r/m mod sib 0 x86))
 
        ((when flg0)
-	(!!ms-fresh :x86-operand-from-modr/m-and-sib-bytes flg0))
+        (!!ms-fresh :x86-operand-from-modr/m-and-sib-bytes flg0))
 
        ((the (signed-byte #.*max-linear-address-size+1*) temp-rip)
-	(+ temp-rip increment-RIP-by))
+        (+ temp-rip increment-RIP-by))
 
        ((when (mbe :logic (not (canonical-address-p temp-rip))
-		   :exec (<= #.*2^47*
-			     (the (signed-byte
-				   #.*max-linear-address-size+1*)
-			       temp-rip))))
-	(!!ms-fresh :temp-rip-not-canonical temp-rip))
+                   :exec (<= #.*2^47*
+                             (the (signed-byte
+                                   #.*max-linear-address-size+1*)
+                               temp-rip))))
+        (!!ms-fresh :temp-rip-not-canonical temp-rip))
 
        ((the (signed-byte #.*max-linear-address-size+1*) addr-diff)
-	(-
-	 (the (signed-byte #.*max-linear-address-size*)
-	   temp-rip)
-	 (the (signed-byte #.*max-linear-address-size*)
-	   start-rip)))
+        (-
+         (the (signed-byte #.*max-linear-address-size*)
+           temp-rip)
+         (the (signed-byte #.*max-linear-address-size*)
+           start-rip)))
        ((when (< 15 addr-diff))
-	(!!ms-fresh :instruction-length addr-diff))
+        (!!ms-fresh :instruction-length addr-diff))
 
-       ;; Raise an error if v-addr is not 16-byte aligned. 
+       ;; Raise an error if v-addr is not 16-byte aligned.
        ;; In case the second operand is an XMM register, v-addr = 0.
        ((when (not (eql (mod v-addr 16) 0)))
         (!!ms-fresh :memory-address-is-not-16-byte-aligned v-addr))
 
        (xmm/mem0 (mbe :logic (part-select xmm/mem :low 0 :high 63)
                       :exec  (the (unsigned-byte 64)
-                                  (logand #uxFFFF_FFFF_FFFF_FFFF xmm/mem))))
+                               (logand #uxFFFF_FFFF_FFFF_FFFF xmm/mem))))
 
        (xmm/mem1 (mbe :logic (part-select xmm/mem :low 64 :high 127)
                       :exec  (the (unsigned-byte 64)
-                                  (logand #uxFFFF_FFFF_FFFF_FFFF (ash xmm/mem -64)))))
+                               (logand #uxFFFF_FFFF_FFFF_FFFF (ash xmm/mem -64)))))
 
        (mxcsr (the (unsigned-byte 32) (mxcsr x86)))
 
@@ -803,7 +765,7 @@
        (result (merge-2-u64s result1 result0))
 
        (mxcsr (the (unsigned-byte 32)
-                   (logior mxcsr0 mxcsr1)))
+                (logior mxcsr0 mxcsr1)))
 
        ;; Update the x86 state:
        (x86 (!mxcsr mxcsr x86))
@@ -811,6 +773,12 @@
        (x86 (!xmmi-size 16 xmm-index result x86))
 
        (x86 (!rip temp-rip x86)))
-      x86))
+      x86)
+
+  :implemented
+  (add-to-implemented-opcodes-table 'SQRTPD #x0F51
+                                    '(:misc
+                                      (eql #.*mandatory-66h* (prefixes-slice :group-3-prefix prefixes)))
+                                    'x86-sqrtpd-Op/En-RM))
 
 ;; ======================================================================
