books/projects/x86isa/machine/instructions/fp/x86-fp-simd-integer-instructions.lisp
@@ -17,66 +17,9 @@
 ; INSTRUCTION: SSE2 64-Bit SIMD Integer Instructions
 ; =============================================================================
 
-(define pcmpeqb32 ((xmm n32p)
-                   (xmm/mem n32p))
-  :inline t
-
-  (let* ((xmm0 (mbe :logic (part-select xmm :low 0 :high 7)
-                    :exec  (the (unsigned-byte 8)
-                             (logand #xFF xmm))))
-         (xmm/mem0 (mbe :logic (part-select xmm/mem :low 0 :high 7)
-                        :exec  (the (unsigned-byte 8)
-                                 (logand #xFF xmm/mem))))
-
-         (xmm1 (mbe :logic (part-select xmm :low 8 :high 15)
-                    :exec  (the (unsigned-byte 8)
-                             (logand #xFF (ash xmm -8)))))
-         (xmm/mem1 (mbe :logic (part-select xmm/mem :low 8 :high 15)
-                        :exec  (the (unsigned-byte 8)
-                                 (logand #xFF (ash xmm/mem -8)))))
-
-         (xmm2 (mbe :logic (part-select xmm :low 16 :high 23)
-                    :exec  (the (unsigned-byte 8)
-                             (logand #xFF (ash xmm -16)))))
-         (xmm/mem2 (mbe :logic (part-select xmm/mem :low 16 :high 23)
-                        :exec  (the (unsigned-byte 8)
-                                 (logand #xFF (ash xmm/mem -16)))))
-
-         (xmm3 (mbe :logic (part-select xmm :low 24 :high 31)
-                    :exec  (the (unsigned-byte 8)
-                             (logand #xFF (ash xmm -24)))))
-         (xmm/mem3 (mbe :logic (part-select xmm/mem :low 24 :high 31)
-                        :exec  (the (unsigned-byte 8)
-                                 (logand #xFF (ash xmm/mem -24)))))
-
-         (byte0 (the (unsigned-byte 8)
-                  (if (int= xmm0 xmm/mem0) #xFF 0)))
-         (byte1 (the (unsigned-byte 8)
-                  (if (int= xmm1 xmm/mem1) #xFF 0)))
-         (byte2 (the (unsigned-byte 8)
-                  (if (int= xmm2 xmm/mem2) #xFF 0)))
-         (byte3 (the (unsigned-byte 8)
-                  (if (int= xmm3 xmm/mem3) #xFF 0)))
-
-         (dword (merge-4-u8s byte3 byte2 byte1 byte0)))
-    dword)
-
-  ///
-
-  (defthm-usb n32p-pcmpeqb32
-    :bound 32
-    :concl (pcmpeqb32 xmm xmm/mem)
-    :gen-type t
-    :gen-linear t))
-
 (def-inst x86-pcmpeqb-Op/En-RM
 
   :parents (two-byte-opcodes fp-opcodes)
-  :implemented
-  (add-to-implemented-opcodes-table 'PCMPEQB #x0F74
-                                    '(:misc
-                                      (eql #.*mandatory-66h* (prefixes-slice :group-3-prefix prefixes)))
-                                    'x86-pcmpeqb-Op/En-RM)
 
   :short "Compare packed bytes for equal"
 
@@ -86,13 +29,69 @@
 
   :returns (x86 x86p :hyp (x86p x86))
 
+  :prepwork
+
+  ((define pcmpeqb32 ((xmm n32p)
+                      (xmm/mem n32p))
+     :inline t
+
+     (let* ((xmm0 (mbe :logic (part-select xmm :low 0 :high 7)
+                       :exec  (the (unsigned-byte 8)
+                                (logand #xFF xmm))))
+            (xmm/mem0 (mbe :logic (part-select xmm/mem :low 0 :high 7)
+                           :exec  (the (unsigned-byte 8)
+                                    (logand #xFF xmm/mem))))
+
+            (xmm1 (mbe :logic (part-select xmm :low 8 :high 15)
+                       :exec  (the (unsigned-byte 8)
+                                (logand #xFF (ash xmm -8)))))
+            (xmm/mem1 (mbe :logic (part-select xmm/mem :low 8 :high 15)
+                           :exec  (the (unsigned-byte 8)
+                                    (logand #xFF (ash xmm/mem -8)))))
+
+            (xmm2 (mbe :logic (part-select xmm :low 16 :high 23)
+                       :exec  (the (unsigned-byte 8)
+                                (logand #xFF (ash xmm -16)))))
+            (xmm/mem2 (mbe :logic (part-select xmm/mem :low 16 :high 23)
+                           :exec  (the (unsigned-byte 8)
+                                    (logand #xFF (ash xmm/mem -16)))))
+
+            (xmm3 (mbe :logic (part-select xmm :low 24 :high 31)
+                       :exec  (the (unsigned-byte 8)
+                                (logand #xFF (ash xmm -24)))))
+            (xmm/mem3 (mbe :logic (part-select xmm/mem :low 24 :high 31)
+                           :exec  (the (unsigned-byte 8)
+                                    (logand #xFF (ash xmm/mem -24)))))
+
+            (byte0 (the (unsigned-byte 8)
+                     (if (int= xmm0 xmm/mem0) #xFF 0)))
+            (byte1 (the (unsigned-byte 8)
+                     (if (int= xmm1 xmm/mem1) #xFF 0)))
+            (byte2 (the (unsigned-byte 8)
+                     (if (int= xmm2 xmm/mem2) #xFF 0)))
+            (byte3 (the (unsigned-byte 8)
+                     (if (int= xmm3 xmm/mem3) #xFF 0)))
+
+            (dword (merge-4-u8s byte3 byte2 byte1 byte0)))
+       dword)
+
+     ///
+
+     (defthm-usb n32p-pcmpeqb32
+       :bound 32
+       :concl (pcmpeqb32 xmm xmm/mem)
+       :gen-type t
+       :gen-linear t)))
+
   :body
   (b* ((ctx 'x86-pcmpeqb-Op/En-RM)
        (r/m (the (unsigned-byte 3) (mrm-r/m  modr/m)))
        (mod (the (unsigned-byte 2) (mrm-mod  modr/m)))
        (reg (the (unsigned-byte 3) (mrm-reg  modr/m)))
-       (lock (eql #.*lock*
-                  (prefixes-slice :group-1-prefix prefixes)))
+       ;; [Shilpi]: The Intel manual doesn't mention that a lock
+       ;; prefix causes an exception for this opcode. Should the
+       ;; following be removed then?
+       (lock (eql #.*lock* (prefixes-slice :group-1-prefix prefixes)))
        ((when lock)
         (!!ms-fresh :lock-prefix prefixes))
 
@@ -111,9 +110,8 @@
             (the (unsigned-byte 128) xmm/mem)
             (the (integer 0 4) increment-RIP-by)
             (the (signed-byte 64) ?v-addr) x86)
-        (x86-operand-from-modr/m-and-sib-bytes #.*xmm-access* 16
-                                               p2 p4? temp-rip
-                                               rex-byte r/m mod sib 0 x86))
+        (x86-operand-from-modr/m-and-sib-bytes
+         #.*xmm-access* 16 p2 p4? temp-rip rex-byte r/m mod sib 0 x86))
 
        ((when flg0)
         (!!ms-fresh :x86-operand-from-modr/m-and-sib-bytes flg0))
@@ -144,40 +142,40 @@
 
        (xmm0 (mbe :logic (part-select xmm :low 0 :high 31)
                   :exec  (the (unsigned-byte 32)
-                              (logand #uxFFFF_FFFF xmm))))
+                           (logand #uxFFFF_FFFF xmm))))
        (xmm/mem0 (mbe :logic (part-select xmm/mem :low 0 :high 31)
                       :exec  (the (unsigned-byte 32)
-                                  (logand #uxFFFF_FFFF xmm/mem))))
+                               (logand #uxFFFF_FFFF xmm/mem))))
 
        (xmm1 (mbe :logic (part-select xmm :low 32 :high 63)
                   :exec  (the (unsigned-byte 32)
-                              (logand #uxFFFF_FFFF (ash xmm -32)))))
+                           (logand #uxFFFF_FFFF (ash xmm -32)))))
        (xmm/mem1 (mbe :logic (part-select xmm/mem :low 32 :high 63)
                       :exec  (the (unsigned-byte 32)
-                                  (logand #uxFFFF_FFFF (ash xmm/mem -32)))))
+                               (logand #uxFFFF_FFFF (ash xmm/mem -32)))))
 
        (xmm2 (mbe :logic (part-select xmm :low 64 :high 95)
                   :exec  (the (unsigned-byte 32)
-                              (logand #uxFFFF_FFFF (ash xmm -64)))))
+                           (logand #uxFFFF_FFFF (ash xmm -64)))))
        (xmm/mem2 (mbe :logic (part-select xmm/mem :low 64 :high 95)
                       :exec  (the (unsigned-byte 32)
-                                  (logand #uxFFFF_FFFF (ash xmm/mem -64)))))
+                               (logand #uxFFFF_FFFF (ash xmm/mem -64)))))
 
        (xmm3 (mbe :logic (part-select xmm :low 96 :high 127)
                   :exec  (the (unsigned-byte 32)
-                              (logand #uxFFFF_FFFF (ash xmm -96)))))
+                           (logand #uxFFFF_FFFF (ash xmm -96)))))
        (xmm/mem3 (mbe :logic (part-select xmm/mem :low 96 :high 127)
                       :exec  (the (unsigned-byte 32)
-                                  (logand #uxFFFF_FFFF (ash xmm/mem -96)))))
+                               (logand #uxFFFF_FFFF (ash xmm/mem -96)))))
 
        (dword0 (the (unsigned-byte 32)
-                    (pcmpeqb32 xmm0 xmm/mem0)))
+                 (pcmpeqb32 xmm0 xmm/mem0)))
        (dword1 (the (unsigned-byte 32)
-                    (pcmpeqb32 xmm1 xmm/mem1)))
+                 (pcmpeqb32 xmm1 xmm/mem1)))
        (dword2 (the (unsigned-byte 32)
-                    (pcmpeqb32 xmm2 xmm/mem2)))
+                 (pcmpeqb32 xmm2 xmm/mem2)))
        (dword3 (the (unsigned-byte 32)
-                    (pcmpeqb32 xmm3 xmm/mem3)))
+                 (pcmpeqb32 xmm3 xmm/mem3)))
 
        (result (merge-4-u32s dword3 dword2 dword1 dword0))
 
@@ -185,61 +183,17 @@
        (x86 (!xmmi-size 16 xmm-index result x86))
 
        (x86 (!rip temp-rip x86)))
-      x86))
+      x86)
 
-(define pmovmskb8 ((xmm n64p))
-  :inline t
-
-  (let* ((bit0  (logbit   7 xmm))
-         (bit1  (logbit  15 xmm))
-         (bit2  (logbit  23 xmm))
-         (bit3  (logbit  31 xmm))
-         (bit4  (logbit  39 xmm))
-         (bit5  (logbit  47 xmm))
-         (bit6  (logbit  55 xmm))
-         (bit7  (logbit  63 xmm))
-
-         (two-bit0 (the (unsigned-byte 2)
-                     (logior (the (unsigned-byte 2) (ash bit1 1))
-                             bit0)))
-         (two-bit1 (the (unsigned-byte 2)
-                     (logior (the (unsigned-byte 2) (ash bit3 1))
-                             bit2)))
-         (two-bit2 (the (unsigned-byte 2)
-                     (logior (the (unsigned-byte 2) (ash bit5 1))
-                             bit4)))
-         (two-bit3 (the (unsigned-byte 2)
-                     (logior (the (unsigned-byte 2) (ash bit7 1))
-                             bit6)))
-
-         (four-bit0 (the (unsigned-byte 4)
-                      (logior (the (unsigned-byte 4) (ash two-bit1 2))
-                              two-bit0)))
-         (four-bit1 (the (unsigned-byte 4)
-                      (logior (the (unsigned-byte 4) (ash two-bit3 2))
-                              two-bit2)))
-
-         (byte (the (unsigned-byte 8)
-                 (logior (the (unsigned-byte 8) (ash four-bit1 4))
-                         four-bit0))))
-    byte)
-
-  ///
-
-  (defthm-usb n08p-pmovmskb8
-    :bound 8
-    :concl (pmovmskb8 xmm)
-    :gen-type t
-    :gen-linear t))
+  :implemented
+  (add-to-implemented-opcodes-table 'PCMPEQB #x0F74
+                                    '(:misc
+                                      (eql #.*mandatory-66h* (prefixes-slice :group-3-prefix prefixes)))
+                                    'x86-pcmpeqb-Op/En-RM))
 
 (def-inst x86-pmovmskb-Op/En-RM
 
   :parents (two-byte-opcodes fp-opcodes)
-  :implemented
-  (add-to-implemented-opcodes-table 'PMOVMSKB #x0FD7
-                                    '(:misc
-                                      (eql #.*mandatory-66h* (prefixes-slice :group-3-prefix prefixes)))
-                                    'x86-pmovmskb-Op/En-RM)
 
   :short "Move byte mask"
 
@@ -251,13 +205,62 @@
 
   :returns (x86 x86p :hyp (x86p x86))
 
+  :prepwork
+
+  ((define pmovmskb8 ((xmm n64p))
+     :inline t
+
+     (let* ((bit0  (logbit   7 xmm))
+            (bit1  (logbit  15 xmm))
+            (bit2  (logbit  23 xmm))
+            (bit3  (logbit  31 xmm))
+            (bit4  (logbit  39 xmm))
+            (bit5  (logbit  47 xmm))
+            (bit6  (logbit  55 xmm))
+            (bit7  (logbit  63 xmm))
+
+            (two-bit0 (the (unsigned-byte 2)
+                        (logior (the (unsigned-byte 2) (ash bit1 1))
+                                bit0)))
+            (two-bit1 (the (unsigned-byte 2)
+                        (logior (the (unsigned-byte 2) (ash bit3 1))
+                                bit2)))
+            (two-bit2 (the (unsigned-byte 2)
+                        (logior (the (unsigned-byte 2) (ash bit5 1))
+                                bit4)))
+            (two-bit3 (the (unsigned-byte 2)
+                        (logior (the (unsigned-byte 2) (ash bit7 1))
+                                bit6)))
+
+            (four-bit0 (the (unsigned-byte 4)
+                         (logior (the (unsigned-byte 4) (ash two-bit1 2))
+                                 two-bit0)))
+            (four-bit1 (the (unsigned-byte 4)
+                         (logior (the (unsigned-byte 4) (ash two-bit3 2))
+                                 two-bit2)))
+
+            (byte (the (unsigned-byte 8)
+                    (logior (the (unsigned-byte 8) (ash four-bit1 4))
+                            four-bit0))))
+       byte)
+
+     ///
+
+     (defthm-usb n08p-pmovmskb8
+       :bound 8
+       :concl (pmovmskb8 xmm)
+       :gen-type t
+       :gen-linear t)))
+
   :body
   (b* ((ctx 'x86-pmovmskb-Op/En-RM)
        (r/m (the (unsigned-byte 3) (mrm-r/m  modr/m)))
        (mod (the (unsigned-byte 2) (mrm-mod  modr/m)))
        (reg (the (unsigned-byte 3) (mrm-reg  modr/m)))
-       (lock (eql #.*lock*
-                  (prefixes-slice :group-1-prefix prefixes)))
+       ;; [Shilpi]: The Intel manual doesn't mention that a lock
+       ;; prefix causes an exception for this opcode. Should the
+       ;; following be removed then?
+       (lock (eql #.*lock* (prefixes-slice :group-1-prefix prefixes)))
        ((when lock)
         (!!ms-fresh :lock-prefix prefixes))
 
@@ -316,6 +319,12 @@
        (x86 (!rgfi-size 8 rgf-index result rex-byte x86))
 
        (x86 (!rip temp-rip x86)))
-      x86))
+      x86)
+
+  :implemented
+  (add-to-implemented-opcodes-table 'PMOVMSKB #x0FD7
+                                    '(:misc
+                                      (eql #.*mandatory-66h* (prefixes-slice :group-3-prefix prefixes)))
+                                    'x86-pmovmskb-Op/En-RM))
 
 ;; ======================================================================
